Java/src/Java/Logic/AssertionLogic.v
@@ -149,15 +149,15 @@ Definition mk_asn (f: Program -> nat -> heap -> Prop)
   (Hheap: forall P k h h', subheap h h' -> f P k h -> f P k h') : asn.
   refine (mkILPreFrm (fun P => mkILPreFrm (fun k => mkILPreFrm (fun h => f P k h) _) _) _).
 Proof.
-  intros P P' HP Hn h H; simpl.
-  eapply HProg; eassumption.
-Grab Existential Variables.
-  assert (forall k' k P h, k' >= k -> f P k' h -> f P k h) as Hnat'.
-  intros k k' P' h Hkk' S.  
-  induction Hkk'. assumption.
-  apply IHHkk'. apply Hnat. assumption.
-  intros n n' Hn'' p S; simpl in *. eapply Hnat'; eassumption.
-  intros h h' Hh H. eapply Hheap; eassumption.
+  + intros t t' Htt' H. apply Hheap with t; [apply Htt' | assumption].
+  + intros k k' Hkk' t H.
+    assert (forall k' k P h, k' >= k -> f P k' h -> f P k h) as Hnat'. {
+      intros m n' P' h Hmn S.  
+      induction Hmn; [assumption|].
+      apply IHHmn. apply Hnat. assumption.
+    }
+    apply Hnat' with k; assumption.
+  + intros P P' HP k h H. eapply HProg; eassumption.
 Defined.
 
 Program Definition pointsto_aux (x : ptr) (f : field) (v : val) : asn :=
